Implemented equality on contexts.

ContextEquality.v
@@ -16,33 +16,187 @@ Notation term := (term F X).
 Notation terms := (vector term).
 Notation context := (context F X).
 
-(*
-   TODO: we might need proof irrelevance here for the
-       H : i = S j + arity f
-   arguments of CFun.
-*)
-
 (* Bisimilarity on contexts *)
 Inductive context_bis : context -> context -> Prop :=
   | Hole_bis : context_bis Hole Hole
-  | CFun_bis : forall f i j H (v v' : terms i) c c' (w w' : terms j),
+  | CFun_bis : forall f i j H H' (v v' : terms i) c c' (w w' : terms j),
                (forall i, term_bis (v i) (v' i)) ->
                context_bis c c' ->
                (forall i, term_bis (w i) (w' i)) ->
-               context_bis (CFun f H v c w) (CFun f H v' c' w').
+               context_bis (CFun f H v c w) (CFun f H' v' c' w').
 
 (* Equality of contexts up to a given depth *)
 Inductive context_eq_up_to : nat -> context -> context -> Prop :=
   | ceut_0    : forall c c' : context, context_eq_up_to 0 c c'
   | ceut_hole : forall n, context_eq_up_to n Hole Hole
-  | ceut_cfun : forall n f i j H (v v' : terms i) c c' (w w' : terms j),
-                (forall i, term_eq_up_to n (v i) (v' i)) ->
-                context_eq_up_to n c c' ->
-                (forall i, term_eq_up_to n (w i) (w' i)) ->
-                context_eq_up_to (S n) (CFun f H v c w) (CFun f H v' c' w').
+  | ceut_cfun : forall d f i j H H' (v v' : terms i) c c' (w w' : terms j),
+                (forall i, term_eq_up_to d (v i) (v' i)) ->
+                context_eq_up_to d c c' ->
+                (forall i, term_eq_up_to d (w i) (w' i)) ->
+                context_eq_up_to (S d) (CFun f H v c w) (CFun f H' v' c' w').
 
 Definition context_eq (c c' : context) :=
-  forall n, context_eq_up_to n c c'.
+  forall d, context_eq_up_to d c c'.
+
+Lemma ceut_fun_inv :
+  forall d f i j H H' (v v' : terms i) c c' (w w': terms j),
+    context_eq_up_to (S d) (CFun f H v c w) (CFun f H' v' c' w') ->
+    context_eq_up_to d c c'.
+Proof.
+intros.
+dependent destruction H0.
+assumption.
+Qed.
+
+Lemma ceut_fun_inv_v :
+  forall d f i j H H' (v v' : terms i) c c' (w w': terms j),
+    context_eq_up_to (S d) (CFun f H v c w) (CFun f H' v' c' w') ->
+    forall i, term_eq_up_to d (v i) (v' i).
+Proof.
+intros.
+dependent destruction H0.
+apply H1.
+Qed.
+
+Lemma ceut_fun_inv_w :
+  forall d f i j H H' (v v' : terms i) c c' (w w': terms j),
+    context_eq_up_to (S d) (CFun f H v c w) (CFun f H' v' c' w') ->
+    forall i, term_eq_up_to d (w i) (w' i).
+Proof.
+intros.
+dependent destruction H0.
+apply H3.
+Qed.
+
+Lemma context_eq_fun_inv :
+  forall f i j H H' (v v' : terms i) c c' (w w': terms j),
+    context_eq (CFun f H v c w) (CFun f H' v' c' w') ->
+    context_eq c c'.
+Proof.
+intros f i j H H' v v' c c' w w' H1 d.
+apply ceut_fun_inv with (1 := H1 (S d)).
+Qed.
+
+Lemma context_eq_fun_inv_v :
+  forall f i j H H' (v v' : terms i) c c' (w w': terms j),
+    context_eq (CFun f H v c w) (CFun f H' v' c' w') ->
+    forall i, term_eq (v i) (v' i).
+Proof.
+intros f i j H H' v v' c c' w w' H1 k d.
+apply ceut_fun_inv_v with (1 := H1 (S d)).
+Qed.
+
+Lemma context_eq_fun_inv_w :
+  forall f i j H H' (v v' : terms i) c c' (w w': terms j),
+    context_eq (CFun f H v c w) (CFun f H' v' c' w') ->
+    forall i, term_eq (w i) (w' i).
+Proof.
+intros f i j H H' v v' c c' w w' H1 k d.
+apply ceut_fun_inv_w with (1 := H1 (S d)).
+Qed.
+
+Lemma context_eq_fun_inv_symbol :
+  forall f i j H (v : terms i) c (w : terms j)
+    f' i' j' H' (v' : terms i') c' (w' : terms j'),
+    context_eq (CFun f H v c w) (CFun f' H' v' c' w') -> f = f'.
+Proof.
+intros.
+assert (H1 := H0 1).
+inversion_clear H1; simpl.
+reflexivity.
+Qed.
+
+Lemma context_eq_fun_inv_i :
+  forall f i j H (v : terms i) c (w : terms j)
+    f' i' j' H' (v' : terms i') c' (w' : terms j'),
+    context_eq (CFun f H v c w) (CFun f' H' v' c' w') -> i = i'.
+Proof.
+intros.
+assert (H1 := H0 1).
+inversion_clear H1; simpl.
+reflexivity.
+Qed.
+
+Lemma context_eq_fun_inv_j :
+  forall f i j H (v : terms i) c (w : terms j)
+    f' i' j' H' (v' : terms i') c' (w' : terms j'),
+    context_eq (CFun f H v c w) (CFun f' H' v' c' w') -> j = j'.
+Proof.
+intros.
+assert (H1 := H0 1).
+inversion_clear H1; simpl.
+reflexivity.
+Qed.
+
+Lemma context_bis_implies_context_eq :
+  forall c c', context_bis c c' -> context_eq c c'.
+Proof.
+intros c c' H d.
+revert c c' H.
+induction d as [| d IHd]; intros c c' H.
+constructor.
+destruct H as [| f i j H H' v v' c c' w w' Hv Hc Hw].
+constructor.
+constructor.
+intro k.
+apply term_bis_implies_term_eq.
+apply Hv.
+apply IHd.
+exact Hc.
+intro k.
+apply term_bis_implies_term_eq.
+apply Hw.
+Qed.
+
+Lemma context_eq_implies_context_bis :
+  forall c c', context_eq c c' -> context_bis c c'.
+Proof.
+induction c as [|f i j H v c IH w]; intros [|f' i' j' H' v' c' w'] H1.
+constructor.
+assert (H2 := H1 1); inversion H2.
+assert (H2 := H1 1); inversion H2.
+assert (H2 := context_eq_fun_inv_symbol H1).
+assert (H3 := context_eq_fun_inv_i H1).
+assert (H4 := context_eq_fun_inv_j H1).
+dependent destruction H2.
+dependent destruction H3.
+dependent destruction H4.
+constructor.
+intro k.
+apply term_eq_implies_term_bis.
+apply (context_eq_fun_inv_v H1).
+apply IH.
+apply (context_eq_fun_inv H1).
+intro k.
+apply term_eq_implies_term_bis.
+apply (context_eq_fun_inv_w H1).
+Qed.
+
+Lemma context_bis_context_eq :
+  forall c c', context_bis c c' <-> context_eq c c'.
+Proof.
+split.
+apply context_bis_implies_context_eq.
+apply context_eq_implies_context_bis.
+Qed.
+
+Lemma context_bis_refl :
+  forall c, context_bis c c.
+Proof.
+(* TODO *)
+Admitted.
+
+Lemma context_bis_symm :
+  forall c c', context_bis c c' -> context_bis c' c.
+Proof.
+(* TODO *)
+Admitted.
+
+Lemma context_bis_trans :
+  forall c1 c2 c3, context_bis c1 c2 -> context_bis c2 c3 -> context_bis c1 c3.
+Proof.
+(* TODO *)
+Admitted.
 
 End ContextEquality.
 
